WIP: Replace Vlists with functions from variables for context interpretations

F_mu/logrel.v
@@ -12,26 +12,118 @@ Section logrel.
   Notation "# v" := (of_val v) (at level 20).
 
   Canonical Structure leibniz_val := leibnizC val.
-
-  Canonical Structure leibniz_le n m := leibnizC (n ≤ m).
+  Canonical Structure leibniz_var := leibnizC var.
 
   
-  Class Val_to_IProp_AlwaysStable (f : leibniz_val -n> iProp lang Σ) :=
-    val_to_iprop_always_stable : ∀ v : val, PersistentP ((cofe_mor_car _ _ f) v).
+  Class Val_to_IProp_Persistent (f : leibniz_val -n> iProp lang Σ) :=
+    val_to_iprop_persistent : ∀ v : val, PersistentP ((cofe_mor_car _ _ f) v).
 
-  Arguments val_to_iprop_always_stable /.
+  Arguments Val_to_IProp_Persistent /.
+
+  (** The empty interpretation used, e.g., in weakening proof *)
+  Definition empty_interp : leibniz_val -n> iProp lang Σ :=
+    {|
+      cofe_mor_car := λ x, False%I
+    |}.
   
+  (** Just to get nicer closed forms, we define extend_context_interp in three steps. *)
+  Program Definition extend_context_interp_fun1
+    (τi : leibniz_val -n> iProp lang Σ)
+    (f : leibniz_var -n> leibniz_val -n> iProp lang Σ) :
+    (leibniz_var -n> leibniz_val -n> iProp lang Σ) :=
+    {| cofe_mor_car :=
+         λ x,
+         match x return leibniz_val -n> iProp lang Σ with
+         | O => τi
+         | S x' => f x'
+         end
+    |}.
+  
+  Program Definition extend_context_interp_fun2
+    (τi : leibniz_val -n> iProp lang Σ) :
+    (leibniz_var -n> leibniz_val -n> iProp lang Σ) -n>
+    (leibniz_var -n> leibniz_val -n> iProp lang Σ) :=
+    {|
+      cofe_mor_car := λ f, extend_context_interp_fun1 τi f
+    |}.
+  Next Obligation.
+  Proof. intros ???? Hfg x; destruct x; cbn; trivial. Qed.
+
+  Program Definition extend_context_interp :
+    (leibniz_val -n> iProp lang Σ) -n>
+    (leibniz_var -n> leibniz_val -n> iProp lang Σ) -n>
+    (leibniz_var -n> leibniz_val -n> iProp lang Σ) :=
+    {|
+      cofe_mor_car := λ τi, extend_context_interp_fun2 τi
+    |}.
+  Next Obligation.
+  Proof. intros n g h H Δ x y. destruct x; cbn; auto. Qed.
+ 
+  
+(*
+  Global Instance extend_context_interp_proper :
+    Proper ((≡) ==> (≡)) extend_context_interp.
+  Proof. intros τ τ' H Δ x; destruct x; cbn; trivial. Qed.
+    
+  Global Instance extend_context_interp_ne n :
+    Proper (dist n ==> dist n) extend_context_interp.
+  Proof. intros τ τ' H Δ x; cbn; destruct x; trivial. Qed.
+*)  
+    
+  Program Definition extend_context_interp_apply :
+    ((leibniz_var -n> leibniz_val -n> iProp lang Σ)) -n>
+    ((leibniz_var -n> leibniz_val -n> iProp lang Σ) -n>
+     leibniz_val -n> iProp lang Σ) -n>
+    (leibniz_val -n> iProp lang Σ) -n> (leibniz_val -n> iProp lang Σ) :=
+    {|
+      cofe_mor_car := λ Δ,
+        {|
+          cofe_mor_car := λ f,
+            {|
+              cofe_mor_car := λ g, f (extend_context_interp g Δ)
+            |}
+        |}
+    |}.
+  Solve Obligations with
+  repeat intros ?; (cbn + idtac);
+    try match goal with [H : _ ≡{_}≡ _|- _] => rewrite H end; trivial.
+  Next Obligation.
+  Proof.
+    intros n Δ Δ' HΔ f g x.  cbn.
+    match goal with
+      |- _ _ ?F x ≡{n}≡ _ _ ?G x =>
+      assert (F ≡{n}≡ G) as HFG; [|rewrite HFG; trivial]
+    end.
+    apply cofe_mor_car_ne; trivial. intros y. cbn.
+    destruct y; trivial.
+  Qed.    
+
   Definition interp_unit : leibniz_val -n> iProp lang Σ :=
     {|
       cofe_mor_car := λ w, (w = UnitV)%I
     |}.
 
-  Definition interp_prod (τ1i τ2i : leibniz_val -n> iProp lang Σ) : leibniz_val -n> iProp lang Σ :=
+  Program Definition interp_prod :
+    (leibniz_val -n> iProp lang Σ) -n> (leibniz_val -n> iProp lang Σ) -n>
+    leibniz_val -n> iProp lang Σ :=
     {|
-      cofe_mor_car := λ w, (∃ w1 w2, w = PairV w1 w2 ∧ ▷ τ1i w1 ∧ ▷ τ2i w2)%I
+      cofe_mor_car :=
+        λ τ1i,
+        {|
+          cofe_mor_car :=
+            λ τ2i,
+            {|
+              cofe_mor_car :=
+                λ w, (∃ w1 w2, w = PairV w1 w2 ∧ ▷ τ1i w1 ∧ ▷ τ2i w2)%I
+            |}
+        |}
     |}.
+  Solve Obligations with
+  repeat intros ?; cbn;
+    repeat apply exist_ne =>?;
+        try match goal with [H : _ ≡{_}≡ _|- _] => rewrite H end; trivial.
 
-  Global Instance interp_prod_proper : Proper ((≡) ==> (≡) ==> (≡)) interp_prod.
+(*  Global Instance interp_prod_proper : Proper ((≡) ==> (≡) ==> (≡)) interp_prod.
   Proof.
     intros τ1 τ1' H1 τ2 τ2' H2 w.
     apply exist_proper =>v. apply exist_proper=> v'.
@@ -44,13 +136,30 @@ Section logrel.
     apply exist_ne =>v. apply exist_ne=> v'.
     repeat apply and_ne; trivial; first [rewrite H1|rewrite H2]; trivial.
   Qed.
+*)
   
-  Definition interp_sum (τ1i τ2i : leibniz_val -n> iProp lang Σ) : leibniz_val -n> iProp lang Σ :=
+  Program Definition interp_sum :
+    (leibniz_val -n> iProp lang Σ) -n> (leibniz_val -n> iProp lang Σ) -n>
+    leibniz_val -n> iProp lang Σ :=
     {|
-      cofe_mor_car := λ w, ((∃ w1, w = InjLV w1 ∧ ▷ τ1i w1) ∨
-                            (∃ w2, w = InjRV w2 ∧ ▷ τ2i w2))%I
+      cofe_mor_car :=
+        λ τ1i,
+        {|
+          cofe_mor_car :=
+            λ τ2i,
+            {|
+              cofe_mor_car :=
+                λ w, ((∃ w1, w = InjLV w1 ∧ ▷ τ1i w1) ∨
+                      (∃ w2, w = InjRV w2 ∧ ▷ τ2i w2))%I
+            |}
+        |}
     |}.
-
+  Solve Obligations with
+  repeat intros ?; cbn; try apply or_ne;
+    try apply exist_ne =>?;
+        try match goal with [H : _ ≡{_}≡ _|- _] => rewrite H end; trivial.
+  
+  (*
   Global Instance interp_sum_proper : Proper ((≡) ==> (≡) ==> (≡)) interp_sum.
   Proof.
     intros τ1 τ1' H1 τ2 τ2' H2 w.
@@ -64,12 +173,29 @@ Section logrel.
     apply or_ne; apply exist_ne =>v;
       apply and_ne; try rewrite H1; try rewrite H2; auto.
   Qed.
-
-  Definition interp_arrow (τ1i τ2i : leibniz_val -n> iProp lang Σ) : leibniz_val -n> iProp lang Σ :=
+*)
+  Program Definition interp_arrow :
+    (leibniz_val -n> iProp lang Σ) -n> (leibniz_val -n> iProp lang Σ) -n>
+    leibniz_val -n> iProp lang Σ :=
     {|
-      cofe_mor_car := λ w, (□ ∀ v, ▷ τ1i v → WP (App (# w) (# v)) @ ⊤ {{τ2i}})%I
+      cofe_mor_car :=
+        λ τ1i,
+        {|
+          cofe_mor_car :=
+            λ τ2i,
+            {|
+              cofe_mor_car :=
+                λ w, (□ ∀ v, ▷ τ1i v → WP (App (# w) (# v)) @ ⊤ {{τ2i}})%I
+            |}
+        |}
     |}.
-
+  Solve Obligations with
+  repeat intros ?; cbn;
+    try apply always_ne;
+    try apply forall_ne=>?; try apply impl_ne; trivial;
+      try apply wp_ne =>?;
+          try match goal with [H : _ ≡{_}≡ _|- _] => rewrite H end; trivial.
+(*    
   Global Instance interp_arrow_proper : Proper ((≡) ==> (≡) ==> (≡)) interp_arrow.
   Proof.
     intros τ1 τ1' H1 τ2 τ2' H2 w.
@@ -85,21 +211,34 @@ Section logrel.
       apply impl_ne;
       [rewrite H1; auto| apply wp_ne; auto].
   Qed.
-  
-  Definition interp_var (k : nat) (x : var) (H : x < k)
-    : (@cofe_Vlist (leibniz_val -n> iProp lang Σ) k) -n> leibniz_val -n> iProp lang Σ :=
-    force_lookup_morph k x H.
-
-  Definition interp_forall (τi : (leibniz_val -n> iProp lang Σ) -n> (leibniz_val -n> iProp lang Σ))
-    : leibniz_val -n> iProp lang Σ :=
+*)  
+  Program Definition interp_forall :
+    ((leibniz_val -n> iProp lang Σ) -n> (leibniz_val -n> iProp lang Σ)) -n>
+    leibniz_val -n> iProp lang Σ :=
     {|
       cofe_mor_car :=
-        λ w,
-        (∃ e, w = TLamV e ∧
-        ∀ (τ'i : {f : (leibniz_val -n> iProp lang Σ) | Val_to_IProp_AlwaysStable f}),
-            □ (▷ WP e @ ⊤ {{λ v, (τi (`τ'i) v)}}))%I
+        λ τi,
+        {|
+          cofe_mor_car :=
+            λ w,
+            (∃ e, w = TLamV e ∧
+                  ∀ (τ'i : {f : (leibniz_val -n> iProp lang Σ) |
+                            Val_to_IProp_Persistent f}),
+                    □ (▷ WP e @ ⊤ {{λ v, (τi (`τ'i) v)}}))%I
+        |}
     |}.
-
+  Next Obligation.
+  Proof.
+    intros τ τ' x y Hxy; cbn. apply exist_ne => e; apply and_ne; auto.
+    rewrite Hxy; trivial.
+  Qed.
+  Next Obligation.
+    intros n f g Hfg x; cbn. apply exist_ne => e; apply and_ne; auto.
+    apply forall_ne=> P.
+    apply always_ne, (contractive_ne _), wp_ne => w.
+    rewrite Hfg; trivial.
+  Qed.    
+(*    
   Global Instance interp_forall_proper : Proper ((≡) ==> (≡)) interp_forall.
   Proof.
     intros τ τ' H1 v; cbn.
@@ -117,15 +256,37 @@ Section logrel.
     apply always_ne, (contractive_ne _), wp_ne=>w.
     rewrite H1; trivial.
   Qed.
-
-  Definition interp_rec_pre
-             (τi : (leibniz_val -n> iProp lang Σ) -n> (leibniz_val -n> iProp lang Σ))
-             (rec_apr : (leibniz_val -n> iProp lang Σ))
-    : (leibniz_val -n> iProp lang Σ) :=
+*)
+  Program Definition interp_rec_pre :
+    ((leibniz_val -n> iProp lang Σ) -n> (leibniz_val -n> iProp lang Σ)) -n>
+    (leibniz_val -n> iProp lang Σ) -n>
+    (leibniz_val -n> iProp lang Σ) :=
     {|
-      cofe_mor_car := λ w, (□ (∃ v, w = FoldV v ∧ ▷ (τi rec_apr v)))%I
+      cofe_mor_car :=
+        λ τi,
+        {| cofe_mor_car :=
+             λ rec_appr,
+             {|
+               cofe_mor_car := λ w, (□ (∃ v, w = FoldV v ∧ ▷ (τi rec_appr v)))%I
+             |}
+        |}
     |}.
+  Next Obligation.
+  Proof.
+    intros τi rec_appr n x y Hxy; rewrite Hxy; trivial.
+  Qed.    
+  Next Obligation.
+  Proof.
+    intros τi n f g Hfg x. cbn.
+    apply always_ne, exist_ne =>w; rewrite Hfg; trivial.
+  Qed.
+  Next Obligation.
+  Proof.
+    intros n τi τi' Hτi f x. cbn.
+    apply always_ne, exist_ne =>w; rewrite Hτi; trivial.
+  Qed.
 
+  (*
   Global Instance interp_rec_pre_proper : Proper ((≡) ==> (≡) ==> (≡)) interp_rec_pre.
   Proof.
     intros τ1 τ1' H1 τ2 τ2' H2 w.
@@ -140,8 +301,7 @@ Section logrel.
     apply always_ne, exist_ne=>e; apply and_ne; trivial.
     apply (contractive_ne _).
     rewrite H1 H2; trivial.
-  Qed.
-  
+  Qed. *)
   Global Instance interp_rec_pre_contr
            (τi : (leibniz_val -n> iProp lang Σ) -n> (leibniz_val -n> iProp lang Σ))
     :
@@ -153,9 +313,18 @@ Section logrel.
     rewrite H; trivial.
   Qed.
   
-  Definition interp_rec (τi : (leibniz_val -n> iProp lang Σ) -n> (leibniz_val -n> iProp lang Σ))
-    := fixpoint (interp_rec_pre τi).
+  Program Definition interp_rec :
+    ((leibniz_val -n> iProp lang Σ) -n> (leibniz_val -n> iProp lang Σ)) -n>
+    (leibniz_val -n> iProp lang Σ)
+    :=
+      {|
+        cofe_mor_car := λ τi, fixpoint (interp_rec_pre τi)
+      |}.
+  Next Obligation.
+  Proof. intros n f g H; apply fixpoint_ne => z; rewrite H; trivial. Qed.
+    
 
+  (*
   Global Instance interp_rec_proper : Proper ((≡) ==> (≡)) interp_rec.
   Proof.
     intros τ τ' H1.
@@ -171,46 +340,28 @@ Section logrel.
     rewrite fixpoint_ne; eauto=>f.
     rewrite H1; trivial.
   Qed.
-
-  Program Fixpoint interp
-           (k : nat) (τ : type) {struct τ}
-    : closed_type k τ → (@cofe_Vlist (leibniz_val -n> iProp lang Σ) k) -n> leibniz_val -n> iProp lang Σ
+*)
+  Program Fixpoint interp (τ : type) {struct τ}
+    : (leibniz_var -n> (leibniz_val -n> iProp lang Σ)) -n> leibniz_val -n> iProp lang Σ
     :=
-        match τ as t return closed_type k t → _ with
-        | TUnit => λ _, {| cofe_mor_car := λ Δ,interp_unit |}
+      match τ with
+        | TUnit => {| cofe_mor_car := λ Δ, interp_unit |}
         | TProd τ1 τ2 =>
-          λ HC',
-          {| cofe_mor_car :=
-               λ Δ,interp_prod
-                     (interp k τ1 (closed_type_prod_1 HC') Δ)
-                     (interp k τ2 (closed_type_prod_2 HC') Δ)|}
-        | TSum τ1 τ2 =>
-          λ HC',
-          {| cofe_mor_car :=
-               λ Δ,interp_sum
-                     (interp k τ1 (closed_type_sum_1 HC') Δ)
-                     (interp k τ2 (closed_type_sum_2 HC') Δ)|}
-        | TArrow τ1 τ2 =>
-          λ HC',
-          {|cofe_mor_car :=
-              λ Δ, interp_arrow
-                     (interp k τ1 (closed_type_arrow_1 HC') Δ)
-                     (interp k τ2 (closed_type_arrow_2 HC') Δ)|}
-        | TVar v => λ HC', {| cofe_mor_car := λ Δ,interp_var k v (closed_type_var HC') Δ |}
+          {| cofe_mor_car := λ Δ, interp_prod (interp τ1 Δ) (interp τ2 Δ)|}
+        | TSum τ1 τ2 => {| cofe_mor_car := λ Δ,interp_sum (interp τ1 Δ) (interp τ2 Δ)|}
+        | TArrow τ1 τ2 => {|cofe_mor_car := λ Δ, interp_arrow (interp τ1 Δ) (interp τ2 Δ)|}
+        | TVar v => {| cofe_mor_car :=
+                        λ Δ : (leibniz_var -n> (leibniz_val -n> iProp lang Σ)), (Δ v) |}
         | TForall τ' =>
-          λ HC',
-          {| cofe_mor_car :=
-               λ Δ,
-               interp_forall
-                 (Vlist_cons_apply Δ (interp (S k) τ' (closed_type_forall HC'))) |}
+          {| cofe_mor_car := λ Δ,
+                             interp_forall (extend_context_interp_apply Δ (interp τ'))|}
         | TRec τ' =>
-          λ HC',
-          {| cofe_mor_car :=
-               λ Δ, interp_rec
-                      (Vlist_cons_apply Δ (interp (S k) τ' (closed_type_rec HC'))) |}
+          {| cofe_mor_car := λ Δ,
+                             interp_rec (extend_context_interp_apply Δ (interp τ'))|}
         end%I.
-  Solve Obligations with repeat intros ?; match goal with [H : _ ≡{_}≡ _|- _] => rewrite H end; trivial.
-
+  Solve Obligations with
+  repeat intros ?; match goal with [H : _ ≡{_}≡ _|- _] => rewrite H end; trivial.
+(*    
   Lemma interp_closed_irrel
         (k : nat) (τ : type) (HC HC': closed_type k τ)
         (Δ : Vlist (leibniz_val -n> iProp lang Σ) k)
@@ -250,7 +401,7 @@ Section logrel.
   Proof.
     rewrite interp_closed_irrel; trivial.
   Qed.
-    
+*)    
   Definition env_subst (vs : list val) (x : var) : expr :=
     from_option (Var x) (of_val <$> vs !! x).
   
@@ -265,44 +416,42 @@ Section logrel.
       by rewrite Hv.
   Qed.
 
-  Class VlistAlwaysStable {k} (Δ : Vlist (leibniz_val -n> iProp lang Σ) k) :=
-    vlistalwaysstable : Forall Val_to_IProp_AlwaysStable (` Δ).
+  Class context_interp_Persistent (Δ : leibniz_var -n> leibniz_val -n> iProp lang Σ) :=
+    contextinterppersistent : ∀ v : var, Val_to_IProp_Persistent (Δ v).
 
-  Global Instance Val_to_IProp_AlwaysStable_Always_Stable
+  Global Instance Val_to_IProp_Persistent_Persistent
            (f : leibniz_val -n> iProp lang Σ)
-           {Hf : Val_to_IProp_AlwaysStable f}
+           {Hf : Val_to_IProp_Persistent f}
            (v : val)
     : PersistentP (f v).
   Proof. apply Hf. Qed.
     
-  Global Instance interp_always_stable
-           k τ H (Δ : Vlist (leibniz_val -n> iProp lang Σ) k)
-           {HΔ : VlistAlwaysStable Δ}
-    : Val_to_IProp_AlwaysStable (interp k τ H Δ).
+  Global Instance interp_Persistent
+         τ (Δ : leibniz_var -n> leibniz_val -n> iProp lang Σ)
+         {HΔ : context_interp_Persistent Δ}
+    : Val_to_IProp_Persistent (interp τ Δ).
   Proof.
-    revert k H Δ HΔ.
-    induction τ; cbn; intros k H Δ HΔ v; try apply _.
+    revert Δ HΔ.
+    induction τ; cbn; intros Δ HΔ v; try apply _.
     - rewrite /PersistentP /interp_rec fixpoint_unfold /interp_rec_pre; cbn.
       apply always_intro'; trivial.
-    - apply (@force_lookup_Forall
-               _ _
-               (λ f : leibniz_val -n> iProp lang Σ, PersistentP (f v))).
-      apply Forall_forall => f H1.
-      eapply Forall_forall in HΔ; [apply HΔ|trivial].
+    - apply Val_to_IProp_Persistent_Persistent; apply HΔ.
   Qed.
 
-  Global Instance alwyas_stable_Δ k Δ Γ vs
-           (Hctx : closed_ctx k Γ)
-           {HΔ : VlistAlwaysStable Δ}
-    : PersistentP (Π∧ zip_with (λ τ v, interp k (` τ) (proj2_sig τ) Δ v) (closed_ctx_list _ Γ Hctx) vs)%I.
+  Global Instance Persistent_context_interp_rel Δ Γ vs
+           {HΔ : context_interp_Persistent Δ}
+    : PersistentP (Π∧ zip_with(λ τ v, interp τ Δ v) Γ vs)%I.
   Proof. typeclasses eauto. Qed.
 
-  Global Instance alwyas_stable_Vlist_cons k f Δ
-           (Hf : Val_to_IProp_AlwaysStable f)
-           {HΔ : VlistAlwaysStable Δ}
-    : VlistAlwaysStable (@Vlist_cons _ k f Δ).
-  Proof. constructor; auto. Qed.
-
+  Global Program Instance extend_context_interp_Persistent f Δ
+           (Hf : Val_to_IProp_Persistent f)
+           {HΔ : context_interp_Persistent Δ}
+    : context_interp_Persistent (@extend_context_interp f Δ).
+  Next Obligation.
+    intros f Δ Hf HΔ v w; destruct v; cbn; trivial.
+    apply HΔ.
+  Qed.
+(*
   Lemma type_context_closed_irrel
         (k : nat) (Δ : Vlist (leibniz_val -n> iProp lang Σ) k) (Γ : list type)
         (vs : list leibniz_val)
@@ -345,7 +494,8 @@ Section logrel.
   Proof.
     rewrite type_context_closed_irrel; trivial.
   Qed.
-
+ *)
+  (*
   Local Ltac ipropsimpl :=
     repeat
       match goal with
@@ -373,75 +523,218 @@ Section logrel.
   Local Hint Extern 2 (_ ⊢ ▷ _)%I => etransitivity; [|rewrite -later_intro] : itauto.
   
   Local Ltac value_case := rewrite -wp_value/= ?to_of_val //; auto 2.
+   *)
 
+  Local Ltac properness :=
+    repeat
+      match goal with
+      | |- (∃ _: _, _)%I ≡ (∃ _: _, _)%I => apply exist_proper =>?
+      | |- (∀ _: _, _)%I ≡ (∀ _: _, _)%I => apply forall_proper =>?
+      | |- (_ ∧ _)%I ≡ (_ ∧ _)%I => apply and_proper
+      | |- (_ ∨ _)%I ≡ (_ ∨ _)%I => apply or_proper
+      | |- (_ → _)%I ≡ (_ → _)%I => apply impl_proper
+      | |- (WP _ {{ _ }})%I ≡ (WP _ {{ _ }})%I => apply wp_proper =>?
+      | |- (▷ _)%I ≡ (▷ _)%I => apply later_proper
+      | |- (□ _)%I ≡ (□ _)%I => apply always_proper
+      end.
 
-  Lemma interp_subst_weaken
-        (k m n : nat)
-        (Δ : Vlist (leibniz_val -n> iProp lang Σ) k)
-        (Ξ : Vlist (leibniz_val -n> iProp lang Σ) m)
-        (ξ : Vlist (leibniz_val -n> iProp lang Σ) n)
+  Lemma interp_unused_contex_irrel
+        (m n : nat)
+        (Δ Δ' : leibniz_var -n> leibniz_val -n> iProp lang Σ)
+        (HΔ : ∀ v, Δ (if lt_dec v m then v else (n + v)) ≡
+                     Δ' (if lt_dec v m then v else (n + v)))
         (τ : type)
-        (HC : closed_type (m + k) τ)
-        (HC' : closed_type (m + (n + k)) τ.[iter m up (ren (+n))])
-    : interp (m + k) τ HC (Vlist_app Ξ Δ)
-             ≡ interp (m + (n + k))
-             τ.[iter m up (ren (+n))] HC' (Vlist_app Ξ (Vlist_app ξ Δ)).
+    :
+      interp τ.[iter m up (ren (+n))] Δ ≡ interp τ.[iter m up (ren (+n))] Δ'.
   Proof.
-    revert k m n Δ Ξ ξ HC HC'.
-    induction τ; intros k m n Δ Ξ ξ HC HC' w; cbn; auto.
-    - apply exist_proper =>w1; apply exist_proper =>w2;
-        repeat apply and_proper; try apply later_proper;
-        solve [trivial|apply IHτ1|apply IHτ2].
-    - apply or_proper; apply exist_proper =>w1;
-        repeat apply and_proper; try apply later_proper;
-        solve [trivial|apply IHτ1|apply IHτ2].
-    - apply always_proper, forall_proper => w1;
-        apply impl_proper; try apply later_proper; try apply wp_proper;
-        solve [apply IHτ1|apply IHτ2].
-    - apply interp_rec_proper =>f; cbn.
-      change (S (m + k)) with (S m + k).
-      change (S (m + (n + k))) with (S m + (n + k)).
+    revert m n Δ Δ' HΔ.
+    induction τ; intros m n Δ Δ' HΔ v; cbn; auto.
+    - properness; trivial; try apply IHτ1; try apply IHτ2; trivial.
+    - properness; trivial; try apply IHτ1; try apply IHτ2; trivial.
+    - properness; trivial; try apply IHτ1; try apply IHτ2; trivial.
+    - match goal with
+        |- _ _ ?f ?x ≡ _ _ ?g ?x =>
+        assert (f ≡ g) as Hfg; [|rewrite Hfg; trivial]
+      end.
+      apply fixpoint_proper => ??; cbn.
+      properness; trivial.
       change (up (iter m up (ren (+n)))) with (iter (S m) up (ren (+n))).
-      rewrite !Vlist_app_cons.
       apply IHτ.
-    - asimpl in *.          
-      revert HC'; rewrite iter_up; intros HC'.
-      destruct lt_dec; asimpl; unfold ids, Ids_type; cbn.
-      + rewrite !force_lookup_l; trivial.
-      + inversion HC'; subst.
-        rewrite force_lookup_r; try lia; intros Hlt.
-        rewrite force_lookup_r; try lia; intros Hlt'.
-        rewrite force_lookup_r; try lia; intros Hlt''.
-        revert Hlt''.
+      {
+        intros x y. destruct x; cbn; trivial.
+        destruct lt_dec.
+        - specialize (HΔ x); destruct lt_dec; auto with omega.
+        - destruct (n + S x) as [|k] eqn:Heq; trivial.
+          specialize (HΔ x); destruct lt_dec; auto with omega.
+          replace (n + x) with k in HΔ by omega; trivial.
+      }
+    -  rewrite iter_up. destruct lt_dec; cbn.
+       + specialize (HΔ x); destruct lt_dec; auto with omega.
+       + asimpl; unfold ids; cbn.
+         specialize (HΔ x); destruct lt_dec; auto with omega.
+         replace (m + n + (x - m)) with (n + x) by omega. trivial.
+    - properness; trivial.
+      change (up (iter m up (ren (+n)))) with (iter (S m) up (ren (+n))).
+      apply IHτ.
+      {
+        intros x y. destruct x; cbn; trivial.
+        destruct lt_dec.
+        - specialize (HΔ x); destruct lt_dec; auto with omega.
+        - destruct (n + S x) as [|k] eqn:Heq; trivial.
+          specialize (HΔ x); destruct lt_dec; auto with omega.
+          replace (n + x) with k in HΔ by omega; trivial.
+      }
+  Qed.
+      
+
+  Program Definition hop_context_interp (m n : nat)
+    (Δ : leibniz_var -n> leibniz_val -n> iProp lang Σ) :
+    (leibniz_var -n> leibniz_val -n> iProp lang Σ) :=
+    {| cofe_mor_car := λ v, if lt_dec v m then Δ v else Δ (v - n) |}.
+
+  Lemma extend_bofore_hop_context_interp (m n : nat)
+        (Δ : leibniz_var -n> leibniz_val -n> iProp lang Σ)
+        (τi : leibniz_val -n> iProp lang Σ)
+        (v : var)
+        (Hv : v > n)
+    :
+      (extend_context_interp τi (hop_context_interp m n Δ) v)
+        ≡ (hop_context_interp (S m) n (extend_context_interp τi Δ) v).
+  Proof.      
+    revert τi Δ n v Hv.
+    induction m; intros τi Δ n v Hv; destruct v; cbn; trivial.
+    replace (S v - n) with (S (v - n)) by omega; trivial.
+    repeat destruct lt_dec; auto with omega.
+    replace (S v - n) with (S (v - n)) by omega; trivial.
+  Qed.
+  
+  Lemma interp_subst_weaken
+        (m n : nat)
+        (Δ : leibniz_var -n> leibniz_val -n> iProp lang Σ)
+        (τ : type)
+    : interp τ Δ ≡ interp τ.[iter m up (ren (+n))] (hop_context_interp m n Δ).
+  Proof.
+    revert m n Δ.
+    induction τ; intros m n Δ v; cbn -[extend_context_interp]; auto.
+    - properness; trivial; try apply IHτ1; try apply IHτ2.
+    - properness; trivial; try apply IHτ1; try apply IHτ2.
+    - properness; trivial; try apply IHτ1; try apply IHτ2.
+    - match goal with
+        |- _ _ ?f ?x ≡ _ _ ?g ?x =>
+        assert (f ≡ g) as Hfg; [|rewrite Hfg; trivial]
+      end.
+      apply fixpoint_proper => ??; cbn -[extend_context_interp].
+      properness; trivial.
+      rewrite IHτ.
+      change (up (iter m up (ren (+n)))) with (iter (S m) up (ren (+n))).
+      apply interp_unused_contex_irrel.
+      {
+      clear. intros [|v]; cbn; trivial.
+      repeat (destruct lt_dec; cbn); auto with omega.
+      destruct (n + S v - n) eqn:Heq1;
+        destruct (n + S v) eqn:Heq2; try destruct lt_dec; auto with omega.
+      match goal with
+        [ |- _ _ _ Δ ?a ≡ _ _ _ Δ ?b] => assert (Heq : a = b) by omega; rewrite Heq; trivial
+      end.
+      }
+    - rewrite iter_up.
+      asimpl; unfold ids; cbn; destruct lt_dec; cbn; destruct lt_dec; auto with omega.
+      replace (m + n + (x - m)) with (x + n) by omega.
+      replace (x + n - n) with x; trivial.
+      { (** An incompleteness in omega and lia! *)
+        clear.
+        replace (x + n) with (n + x) by omega.
+        induction n; cbn; auto with omega.
+        induction x; cbn; trivial.
+      }      
+    - properness; trivial.
+      change (up (iter m up (ren (+n)))) with (iter (S m) up (ren (+n))).
+      rewrite IHτ.
+      apply interp_unused_contex_irrel.
+      {
+        clear. intros [|v]; cbn; trivial.
+        repeat (destruct lt_dec; cbn); auto with omega.
+        destruct (n + S v - n) eqn:Heq1;
+          destruct (n + S v) eqn:Heq2; try destruct lt_dec; auto with omega.
         match goal with
-          [|- ∀ _, _ (force_lookup _ ?A _) _ ≡ _ (force_lookup _ ?B _) _] =>
-          replace B with A by lia; intros Hlt''
+          [ |- _ _ _ Δ ?a ≡ _ _ _ Δ ?b] => assert (Heq : a = b) by omega; rewrite Heq; trivial
         end.
-        rewrite force_lookup_proper; eauto.
-    - apply exist_proper =>w1; apply and_proper; auto.
-      apply forall_proper; intros [f Hf].
-      apply always_proper, later_proper, wp_proper => w2.
-      cbn.
-      change (S (m + k)) with (S m + k).
-      change (S (m + (n + k))) with (S m + (n + k)).
-      change (up (iter m up (ren (+n)))) with (iter (S m) up (ren (+n))).
-      rewrite !Vlist_app_cons.
-      apply IHτ.
+      }
   Qed.
 
   Lemma interp_ren_S (k : nat) (τ : type)
-        (Δ : Vlist (leibniz_val -n> iProp lang Σ) k)
+        (Δ : leibniz_var -n> leibniz_val -n> iProp lang Σ)
         (τi : leibniz_val -n> iProp lang Σ)
-        (HC : closed_type k τ) (HC' : closed_type (S k) τ.[ren (+1)])
         (v : leibniz_val)
-    : interp k τ HC Δ v ≡ interp (S k) τ.[ren (+1)] HC' (Vlist_cons τi Δ) v.
+    : interp τ Δ v ≡ interp τ.[ren (+1)] (extend_context_interp τi Δ) v.
   Proof.
-    rewrite -(Vlist_nil_app Δ).
-    rewrite (Vlist_app_cons τi Vlist_nil Δ).
-    rewrite -(Vlist_nil_app (Vlist_app (Vlist_cons τi Vlist_nil) Δ)).
-    apply (interp_subst_weaken k 0 1).
+    rewrite (interp_subst_weaken 0 1).
+    apply interp_unused_contex_irrel.
+    { clear. intros [|v]; cbn; trivial. }
   Qed.
 
+  Lemma interp_subst_iter_up
+        (m : nat)
+        (Δ : leibniz_var -n> leibniz_val -n> iProp lang Σ)
+        (τ : type)
+        (τ' : type)
+    : interp τ
+             (iter m (extend_context_interp empty_interp)
+                   (extend_context_interp (interp τ' Δ) Δ))
+             ≡ interp τ.[iter m up (τ' .: ids)] 
+                          (iter m (extend_context_interp empty_interp) Δ).
+  Proof.
+    revert m Δ.
+    induction τ; intros m Δ v; cbn -[extend_context_interp]; auto.
+    - properness; trivial; try apply IHτ1; try apply IHτ2.
+    - properness; trivial; try apply IHτ1; try apply IHτ2.
+    - properness; trivial; try apply IHτ1; try apply IHτ2.
+    - match goal with
+        |- _ _ ?f ?x ≡ _ _ ?g ?x =>
+        assert (f ≡ g) as Hfg; [|rewrite Hfg; trivial]
+      end.
+      apply fixpoint_proper => ??; cbn -[extend_context_interp].
+      properness; trivial.
+      
+      rewrite IHτ.
+      change (up (iter m up (ren (+n)))) with (iter (S m) up (ren (+n))).
+      apply interp_unused_contex_irrel.
+      {
+      clear. intros [|v]; cbn; trivial.
+      repeat (destruct lt_dec; cbn); auto with omega.
+      destruct (n + S v - n) eqn:Heq1;
+        destruct (n + S v) eqn:Heq2; try destruct lt_dec; auto with omega.
+      match goal with
+        [ |- _ _ _ Δ ?a ≡ _ _ _ Δ ?b] => assert (Heq : a = b) by omega; rewrite Heq; trivial
+      end.
+      }
+    - rewrite iter_up.
+      asimpl; unfold ids; cbn; destruct lt_dec; cbn; destruct lt_dec; auto with omega.
+      replace (m + n + (x - m)) with (x + n) by omega.
+      replace (x + n - n) with x; trivial.
+      { (** An incompleteness in omega and lia! *)
+        clear.
+        replace (x + n) with (n + x) by omega.
+        induction n; cbn; auto with omega.
+        induction x; cbn; trivial.
+      }      
+    - properness; trivial.
+      change (up (iter m up (ren (+n)))) with (iter (S m) up (ren (+n))).
+      rewrite IHτ.
+      apply interp_unused_contex_irrel.
+      {
+        clear. intros [|v]; cbn; trivial.
+        repeat (destruct lt_dec; cbn); auto with omega.
+        destruct (n + S v - n) eqn:Heq1;
+          destruct (n + S v) eqn:Heq2; try destruct lt_dec; auto with omega.
+        match goal with
+          [ |- _ _ _ Δ ?a ≡ _ _ _ Δ ?b] => assert (Heq : a = b) by omega; rewrite Heq; trivial
+        end.
+      }
+    
+
+
+    
   Lemma interp_subst_iter_up
         (k m : nat)
         (Δ : Vlist (leibniz_val -n> iProp lang Σ) k)
@@ -541,5 +834,5 @@ Section logrel.
     - apply interp_ren_S.
     - apply IHΓ.
   Qed.
-
+*)
 End logrel.
